backends/lean/Aeneas/Std/Scalar/Core.lean
@@ -626,14 +626,15 @@ theorem UScalar.tryMk_eq_DELETE_THIS_PROBABLY (ty : UScalarTy) (x : Nat) :
     grind
 
 theorem UScalar.tryMk_eq (ty : UScalarTy) (x : Nat) :
-  (tryMk ty x).match_dep
-    (fun y => y.val = x ∧ inBounds ty x)
-    (fun _e => ¬ (inBounds ty x))
-    (fun _ => False)
+  match (tryMk ty x).match with
+    | .ok y => y.val = x ∧ inBounds ty x
+    | .vis (.fail _e) _k => ¬ (inBounds ty x)
+    | _ => False
   := by
   have := UScalar.tryMkOpt_eq ty x
   simp [tryMk, ofOption]
   cases h: tryMkOpt ty x <;> simp_all
+  --
 
 -- TODO: delete old one
 -- theorem UScalar.tryMk_eq (ty : UScalarTy) (x : Nat) :
@@ -672,10 +673,10 @@ theorem IScalar.tryMkOpt_eq (ty : IScalarTy) (x : Int) :
 --     grind
 
 theorem IScalar.tryMk_eq (ty : IScalarTy) (x : Int) :
-  (tryMk ty x).match_dep
-  (fun y => y.val = x ∧ inBounds ty x)
-  (fun _e => ¬ (inBounds ty x))
-  (fun _ => False)
+  match (tryMk ty x).match with
+  | .ok y => y.val = x ∧ inBounds ty x
+  | .vis (.fail _e) _k => ¬ (inBounds ty x)
+  | _ => False
   := by
   have := tryMkOpt_eq ty x
   simp [tryMk]
